\section{2022-10-26}

\noindent
Last time: \\
Moran's theorem for fractals \\

\noindent
Today: \\
Return to rudin Narrative following chapter $3$: $L^{p}$-spaces.

\subsection{$L^{p}$-spaces}

Recall definition of $L^{1}$.

$m$ is a measure on $\sigma$-algebra $S$ on a set $X$.

$\mathcal{L}^{1}(m)$ is the space of measurable $f : [-\infty, \infty]$ such that

\begin{align*}
	[f]_{\mathcal{L}^{1}(m)} = \int |f| dm < \infty
\end{align*}

let $\mathcal{N}(m) = \{f : X \to [-\infty, \infty] \text{ meas }: m(\{x : f(x) \neq 0\} = 0\}$ be the set of functions that vanish away from a set of measure zero,

Observe
\begin{align*}
	[f]_{\mathcal{L}^1 (m) } = 0 \text{ for } f \in \mathcal{N}(m) \\
\end{align*} let
 \begin{align*}
	 L^{1} (m) &= \mathcal{L}^1 (m) / \mathcal{N} (m) \\
	 \|\{f\}\|_{L^1 (m) } &= \|f\|_{\mathcal{L}^1 (m) } 
\end{align*} 


\subsection{ Jensen's Inequality }
	
\begin{definition}[Convex]
	$\phi : \R \to \R$ is convex if and only if
	\begin{align*}
		\phi (( 1 - t) a + tb) \leq (1-t) \phi (a) + t \phi (b)
	\end{align*} for $a \leq b$ and $0 \leq t \leq 1$

	equivalently, 
	\begin{align*}
		\frac{\phi (c) - \phi (a)}{c - a} \leq \frac{\phi (b) - \phi (c)}{b - c} 
		\quad \text{for} \quad  a < b
	\end{align*} 
\end{definition}
	
\begin{lemma}
	Convex $\implies$ continuous
\end{lemma}

\begin{proof}
	$a < x < y_{k+1} < y_{k}$ where $y_{k} \xrightarrow[k \to \infty]{} \infty$ then
	\begin{align*}
		\frac{\phi(x) - \phi(a)}{x - a} &\leq \frac{\phi(y_{k+1}) - \phi (x)}{y_{k+1} - x} \\
										&\leq \frac{\phi(y_{k} - \phi(x)}{y_{k} - x}
	\end{align*} then
	\begin{align*}
		\frac{\phi(y_{k} - \phi(x)}{y_{k} - x} \to \alpha \quad \text{as} \quad k \to \infty \quad \text{and} \\
		\phi(y) = \phi(x) + \alpha (y - x) + \mathcal{O}( | y -x|) \quad \text{for} \quad y > x
	\end{align*} 
\end{proof}

\begin{remark}
	we could extend the notion of convexity to allow $\phi : [-\infty, \infty] \to (-\infty, \infty]$ 
	\begin{lemma}
		okay except for jumps [insert pic]
		\begin{align*}
			f(x) =
			\begin{cases}
				\infty & |x| > 1 \\
				0 &|x| \leq 1
			\end{cases}
		\end{align*} 
	\end{lemma}
	
\end{remark}

\begin{theorem}[Jensen's Inequality]
	$m(x) = 1$, $f \in C^{1}(m)$, $a < f < b$ and \\ 
	$\phi : (a,b) \to \R$ convex, then
	\begin{align*}
		\phi\left(\int f dm \right) \leq \int \phi(f) dm
	\end{align*} 
\end{theorem}

\begin{proof}
	Let $c = \int f dm$. Choose $\alpha \in \R$ so
	\begin{align*}
		\phi (x) \geq \phi (c) + \alpha (x - c) \quad x \in (a,b)
	\end{align*} 
	compute
	\begin{align*}
		\int \phi (f) dm &\geq \int \phi (c) + \alpha (f -c) dm \\
						 &= \phi (c) \int 1 dm + \alpha \int f dm - \alpha c \int 1 dm \\
						 &= \phi (c) + \alpha c - \alpha \\
						 &= \phi (c) = \phi \left( \int f dm \right)
	\end{align*}
\end{proof}

\begin{example}[Arithmatic - geometric mean inequality]
	$e^{x}$ convex
	($\frac{d^{2}}{dx^{2}} e^{x} = e^{x} \geq 0$ or $e^{x} = \sum \frac{x^{k}}{k!} =$ sum of convexterms.
\end{example}

\begin{align*}
	e^{\int f dm} \leq \int e^{f} dm \\
	e^{\log f dm} \leq \int f dm \quad f > 0 \\ 
\end{align*} let $m$ be the $\frac{1}{N} \times$ counting measure on $\{1, \ldots, N \}$ 

\begin{align*}
	e^{\frac{1}{N} \log f_{1} + \cdots + \log f_{N}} \leq \frac{1}{N} (f_{1} + \cdots + f_{N} ) \\
	(f_{1}, \ldots, f_{N})^{\frac{1}{N}} \leq \frac{f_{1} + \cdots + f_{N}}{N} \quad \text{for} \quad f_{1}, \ldots, f_{N} > 0
\end{align*} 

\begin{theorem}[Holder Inequality]
	Suppose $1 < p,q < \infty$ and $\frac{1}{p} + \frac{1}{q} = 1$.
	By convexity,
	\begin{align*}
		e^{\frac{s}{p} + \frac{t}{q}} \leq \frac{e^{s}}{p} + \frac{e^{t}}{q}
	\end{align*} 
\end{theorem}

\begin{remark}
	If $0 < a,b < \infty$, then letting $s = pbqa$ and $t = qbga$ [check]?
	gives
	\begin{align*}
		ab \leq \frac{a^{p}}{p} + b^{q}
	\end{align*} also true for $0 \leq a,b \leq \infty$
\end{remark}

\begin{theorem}[Holder]
	If $f,g: X \to [0,\infty]$ measurable, then 
	 \begin{align*}
		\int fg dm \leq \left( \int f^{p} dm\right)^{\frac{1}{p}} \left( \int g^{q} dm\right)^{\frac{1}{q}}
	\end{align*} 
\end{theorem}

\begin{proof}
	Assume $f,g \notin \mathscr{N}(m)$
\end{proof}


