\section{2022-11-16}

Last lecture we discussed several theorems:

\begin{theorem}[Absolute Continuity of Functions]
A $f : [a,b] \to \R$  is \underline{absolutely} \underline{continuous} if and only if for $\varepsilon > 0$, there is $\delta > 0$ so that
	\begin{align*}
		\sum_{k=1} | f (b_k) - f(a_k) | < \varepsilon \quad \text{whenever} \\
		a \leq a_k \leq b_k \leq k_{k+1} \leq b_{k+1} \leq b
	\end{align*} and
	\begin{align*}
		\sum_{k=1}^{n} | b_k - a_k | < \delta
	\end{align*}
\end{theorem}

\begin{lemma}
	Absolutely continuous implies continuous.
\end{lemma}

Note the reverse is not true

\begin{example}
	If $C \subseteq [0,1]$ is he $1/3$ cantor set and
	\begin{align*}
		F(x) = \int \1_{[0,x] \cap C} dH^{\frac{\log{2}}{\log{3}}}
	\end{align*} then $F$ is continuous but NOT absolutely continous.
\end{example}


\begin{theorem}
	$F : [a,b] \to \R$ is absolutely continous if and only if
	\begin{align*}
		F(x) - F(0) = \int \1_{[0,x]} f dL \quad \text{for some } f \in L^{1} ([0,1])
	\end{align*}
\end{theorem}

To prove this we need three lemmas:

\begin{lemma}
	If $f : [a,b] \to \R$ is absolutely continuous and
	\begin{align*}
		\bar{f} (x) = \sup\{ \sum_{k=1}^{n} | f (y_k) - f (y_{k-1}) | : a = y_0 \leq y_1 \leq \ldots \leq y_n = x \}
	\end{align*}
	Then $f_{\pm} - \frac{1}{2} (\bar{f} \pm f)$ are absolutely continuous and non-decreasing.
\end{lemma}

\begin{notation}
	Call $\bar{f}$ the total variation of $f$.
\end{notation}

\begin{proof}
	Adding a new point, $\tilde{y}$, to $\{y_{k}\}$, then
	\begin{align*}
		y_0 \leq \ldots \leq y_k \leq \tilde{y} \leq y_{k+1} \leq \ldots \leq y_n
	\end{align*}
	Then adding this point will only increase
	\begin{align*}
		\sum_{k=1}^n | f( y_k) - f(y_{k-1}) |
	\end{align*}

	If $a \leq x \leq y \leq b$ then
	\begin{align*}
		\bar{f} (y) - \bar{f}(x) &= \sup \{\sum_{k=1}^{n} |f (z_k) - f (z_{k - 1}) | : x = z_0 \leq \ldots \leq z_n = y \} \\
								 &\geq | f(y) - f(x) |
	\end{align*}
	If $a \leq x \leq y \leq b$ then
	 \begin{align*}
		 f_{\pm} (y) - f_{\pm} (x) &= \bar{f} (y) - \bar{f} (x) \pm | f(y) - f(x) | \\
								   &\geq |f(y) - f(x) | - | f(y) - f(x)| \\
								   &= 0
	\end{align*}
	Fix $\varepsilon > 0$, since $f$ is absolutely continuous, there is a $\delta > 0$ so
	\begin{align*}
		\sum_{k=1}^n | f (b_{k}) - f (a_k) | < \varepsilon/2
	\end{align*} when
	\begin{align*}
		\sum_{k=1}^n (b_k - a_k) < \delta \quad \text{and} \quad a \leq a_k \leq b_k \leq a_{k+1} \leq b_{k+1} \leq b
	\end{align*}


	Now suppose $a \leq a_k \leq b_k \leq a_{k+1} \leq b_{k+1} \leq b$
	and
	\begin{align*}
		\sum_{k+1}^n (b_k - a_k) < \delta
	\end{align*}
	for each $k$, choose
	\begin{align*}
		a_k = y_{k,1} \leq \ldots \leq y_{k, m} = b_k
	\end{align*} so that
	\begin{align*}
		0 \leq \bar{f}(b_k) - \bar{f} (a_k) \leq \frac{\varepsilon}{2^{n}} + \sum_{j=1}^m |f(y_{k,j}) - f(y_{k, j-1}) |
	\end{align*}
	Since
	\[
		\sum_{k,j} y_{k,j} - y_{k,j+2} | < \delta \\
	\] and
	\[
		(y_{k, j-1}, y_{k,j})
	\] disjoint.

	Now by absolute continuity:
	\begin{align*}
		\sum_{k=1}^{n} | \bar{f}(b_k) - \bar{f}(a_k) | &\leq \frac{\varepsilon}{2} + \sum_{k,j} |f (y_{k,j}) - f(y_{k,j-1}) | \\
													   &\leq \frac{\varepsilon}{2} + \frac{\varepsilon}{2}
	\end{align*}

\end{proof}

\begin{example}[Counter example]
	consider $f(x) = x^{2} \sin(\frac{1}{x^2})$ and let $f(0) = 0$.
	Observe $f$ is everywhere differentiable and
	\[
		f'(x) = 2x \sin(\frac{1}{x^{2}}) - \frac{2}{x} \cos(\frac{1}{x^2})
	\] (the second term dominates near zero).

	For $x \neq 0$ and $f'(0) = 0$
	\[
		\int | f'(x) | \1_{[-1, 1]} dL = \infty
	\]
	it's impossible to write $f = f_{+} - f_{-}$ with $f_{\pm}$ continuous and non-decreasing.
\end{example}


\begin{lemma}
	If $f : [a,b] \to \R$ is absolutely continuous and non-decreasing, then
	\begin{align*}
		F(x) - F(0) = \int \1_{[0,x)} f dL \quad \text{where} \quad f \in L^1 ([0,1])
	\end{align*}
\end{lemma}

\begin{proof}
	Assume $[a,b] = [0,1]$.
	let
	 \[
		G(x) = \frac{F(x) - F(0) + x}{F(1) - F(0) + 1}
	\].
	Observe $G$ is absolutely continuous and $G$ is an increasing bijection $G [0,1] \to [0,1]$ (check).

	It follows that $G$ is continuous and increasing and $A \subseteq [0,1]$, borel if and only if $G(A)$, is Borel.

	Define Borel measure $m$ on $[0,1]$ by
	\[
		m(A) = L(G(A))
	\].
	Since $G$ is a bijection, $m$ is a measure. (in particular, $m$ is countably additive).
	\begin{claim}
		$m << L$
	\end{claim}
	Suppose $L(A) = 0$, then choose $U \contains A$ open with $L(U) < \delta$.
	$U$ is union of disjoint intervals, since we are working on $\R.$
	And since  $G$ is absolutely continuous
	\[
		L(G(U)) < \varepsilon \delta
	\] where $\varepsilon \delta \to 0$ as $\delta \to 0$.
	So
	\[
		m(A) = L(G(A)) \leq L(G(U)) \leq \varepsilon \delta \to 0
	\] as $\delta \to 0$ and so $m(A) = 0$.

	By Radon-Nikodym,
	\begin{align*}
		m(A) &= \int \1_{A} g dL  \quad \text{with} \quad g \in L^1 ([0,1]) \\
		\int \1_{[0,x]} g dL &= m([0,x]) = L(G([0,x])) = L([G(0), G(x)]) = G(x)
	\end{align*}
	Let
	\[
		f = (F(1) - F(0) + 1 ) g - 1.
	\]then
	\[
		f \in L^1([0,1])
	\] and
	\[
		\int \1_{[0,x]} f dL = F(x) - F(0)
	\]
\end{proof}

\begin{lemma}
	If $m_1, m_2 : S \to [0, \infty)$ measures and
	 $m_1 << m_2$, then for $\varepsilon > 0$, there is $\delta > 0$ so
	 \[
	 	m_2(A) < \delta \implies m_1 (A) < \varepsilon
	 \]
\end{lemma}

\begin{proof}
	Suppose for contradiction that the conclussion fails,
	then there is $\varepsilon > 0 $ and $A_n \in S$ with
	\[
		m_1 (A_{n}) \geq \varepsilon \quad \text{and} \quad m_2 (A_n) \leq 2^{-n}
	\]
	Let
	\[
		B = \bigcap_{n \geq 1} \bigcup_{m \geq n} A_m
	\]

	\underline{Compute}:
	\[
		m(B) = \lim_{n \to \infty} m_1 ( \bigcup_{m \geq n} A_m ) \geq \varepsilon
	\] and
	\begin{align*}
		m_2 (B) &= \lim_{n \to \infty} m_2 (\bigcup_{m \geq n} A_M ) \\
				&= \lim_{n \to \infty} 2^{1 - n}
	\end{align*} so $m_1 <\nless m_2 = 0$.
\end{proof}

Finally we can proceed to the proof of the original theorem:

\begin{proof} We follow several steps:
	\begin{enumerate}
		\item[step 1:]
			Suppose $F : [a,b] \to \R$ is absolutely continuous, then
			\begin{enumerate}
				\item[By Lemma 1:] $F = f_{+} - F_{-}$ where
					$F_{\pm} : [a,b] \to \R$ are absolutely continuous and non-decreasing.

				\item[By Lemma 2:]
					\[
					F_{\pm}(x) - F_{\pm} (0) = \int \1_{[0,x]} f_{\pm} dL \quad \text{with} \quad f_{\pm} \in L^1([0,1])
				\] now
				\[
					F(x) - F(0) = \int \1_{[0,x]} (F_{+} - f_{-} ) dL \\
				\]
				and
				\[
					f_{+} - f_{-} \in L^1([0,1]).
				\]
			\end{enumerate}

		\item[step 2:]
			Suppose
			\[
					F(x) - F(0) = \int \1_{[0,x]} f dL \quad \text{with} \quad f \in L^1([0,1])
			\]
			let $f_{\pm} = \max\{0, \pm f\}$


			Define $m_{\pm}$ by $dm_{\pm} = f_{\pm} dL$. Since $m_{\pm} << L$, givem $\varepsilon > 0,$ there is $\delta$ so
			\[
				L(A) < \delta \implies m_{\pm}(A) < \varepsilon.
			\]
			This implies
			\[
				F_{\pm}(x) = \int \1_{[0,1]} f_{\pm} dL
			\]
			are absolutely continous.

			If
			\begin{align*}
									&\sum (b_k - a_k) < \delta \\
					\text{and} \qquad &a_{k} \leq b_k \leq a_{k+1} \leq b_{k+1}
			\end{align*}

			then
			 \[
				\sum | f_{\pm}(b_k) - F_{\pm}(a_k) | = m_{\pm} ( \cup_{k} (a_k, b_k) < \varepsilon
			\]
			and since $F(x) - F(0) = F^{+} (x) - F^{-} (x)$,
			$F$ is also absolutely continuous.
	\end{enumerate}

\end{proof}

Next ime we will cover product measures and Fubini.

We finished lecture by discussing midterm 2.
